Insertion sort progress

examples/Examples/ProgramsProofs/InsertionSort.lean
@@ -9,32 +9,77 @@ end expect
 
 
 
+expect error {{{ insertSortedNoProof }}}
+  def insertSorted [Ord α] (arr : Array α) (i : Fin arr.size) : Array α :=
+    match i with
+    | ⟨0, _⟩ => arr
+    | ⟨i' + 1, _⟩ =>
+      have : i' < arr.size := by
+        skip
+      match Ord.compare arr[i'] arr[i] with
+      | .lt | .eq => arr
+      | .gt =>
+        insertSorted (arr.swap ⟨i', by assumption⟩ i) ⟨i', by simp [*]⟩
+message
+"unsolved goals
+α : Type ?u.7
+inst✝ : Ord α
+arr : Array α
+i : Fin (Array.size arr)
+i' : Nat
+isLt✝ : i' + 1 < Array.size arr
+⊢ i' < Array.size arr"
+end expect
 
--- #eval swap aPair
+
+expect info {{{ lt_of_succ_lt_type }}}
+  #check Nat.lt_of_succ_lt
+message
+"Nat.lt_of_succ_lt {n m : Nat} (a✝ : Nat.succ n < m) : n < m"
+end expect
 
 -- Precondition: array positions 0 .. i-1 are sorted
 -- Postcondition: array positions 0 .. i are sorted
-def insertSorted [Ord α] (arr : Array α) (i : Nat) (_ : i < arr.size) : Array α :=
-  match i with
-  | 0 => arr
-  | i' + 1 =>
-    have : i' < arr.size := by
-      simp [Nat.lt_of_succ_lt, *]
-    match Ord.compare arr[i'] arr[i' + 1] with
-    | .lt | .eq => arr
-    | .gt =>
-      let j : Fin arr.size := ⟨i', by assumption⟩
-      let j' : Fin arr.size := ⟨i' + 1, by assumption⟩
-      insertSorted (arr.swap j j') i' (by simp [*])
+book declaration {{{ insertSorted }}}
+  def insertSorted [Ord α] (arr : Array α) (i : Fin arr.size) : Array α :=
+    match i with
+    | ⟨0, _⟩ => arr
+    | ⟨i' + 1, _⟩ =>
+      have : i' < arr.size := by
+        simp [Nat.lt_of_succ_lt, *]
+      match Ord.compare arr[i'] arr[i] with
+      | .lt | .eq => arr
+      | .gt =>
+        insertSorted (arr.swap ⟨i', by assumption⟩ i) ⟨i', by simp [*]⟩
+stop book declaration
 
-partial def insertionSortLoop [Ord α] (arr : Array α) (i : Nat) : Array α :=
+
+theorem insert_sorted_size_eq [Ord α] (len : Nat) (i : Nat) : (arr : Array α) → (isLt : i < arr.size) → (arr.size = len) → (insertSorted arr ⟨i, isLt⟩).size = len := by
+  induction i with
+  | zero =>
+    intro arr isLt hLen
+    simp [insertSorted, *]
+  | succ i' ih =>
+    intro arr isLt hLen
+    simp [insertSorted]
+    split <;> simp [*]
+
+def insertionSortLoop [Ord α] (arr : Array α) (i : Nat) : Array α :=
   if h : i < arr.size then
-    insertionSortLoop (insertSorted arr i h) (i + 1)
+    have size_eq : (insertSorted arr { val := i, isLt := h }).size = arr.size := by
+      apply insert_sorted_size_eq arr.size i arr h rfl
+    have : (insertSorted arr { val := i, isLt := h }).size - (i + 1) < arr.size - i := by
+      rw [size_eq]
+      simp [Nat.sub_succ_lt_self, *]
+    insertionSortLoop (insertSorted arr ⟨i, h⟩) (i + 1)
   else
     arr
+termination_by insertionSortLoop arr i => arr.size - i
 
 def insertionSort [Ord α] (arr : Array α) : Array α :=
   insertionSortLoop arr 0
+
+#eval insertionSort #[3, 1, 7, 4]
 
 -- namespace Instrumented
 
