examples/Examples/ProgramsProofs/Fin.lean
@@ -1,1 +1,87 @@
 import Examples.Support
+
+namespace FinDef
+
+book declaration {{{ Fin }}}
+  structure Fin (n : Nat) where
+    val  : Nat
+    isLt : LT.lt val n
+stop book declaration
+
+
+
+end FinDef
+
+
+expect info {{{ fiveFinEight }}}
+  #eval (5 : Fin 8)
+message
+"5"
+end expect
+
+
+expect info {{{ finOverflow }}}
+  #eval (45 : Fin 10)
+message
+"5"
+end expect
+
+def Fin.next? (i : Fin n) : Option (Fin n) :=
+  if h : i.val + 1 < n then
+    some ⟨i.val + 1, h⟩
+  else
+    none
+
+
+expect info {{{ nextThreeFin }}}
+  #eval (3 : Fin 8).next?
+message
+"some 4"
+end expect
+
+
+expect info {{{ nextSevenFin }}}
+  #eval (7 : Fin 8).next?
+message
+"none"
+end expect
+
+
+
+namespace Finny
+
+book declaration {{{ ArrayFindHelper }}}
+  def findHelper (arr : Array α) (p : α → Bool) (i : Nat) : Option (Fin arr.size × α) :=
+    if h : i < arr.size then
+      let x := arr[i]
+      if p x then
+        some (⟨i, h⟩, x)
+      else findHelper arr p (i + 1)
+    else none
+  termination_by findHelper arr p i => arr.size - i
+stop book declaration
+
+book declaration {{{ ArrayFind }}}
+  def Array.find (arr : Array α) (p : α → Bool) : Option (Fin arr.size × α) :=
+    findHelper arr p 0
+stop book declaration
+
+
+  def arrayMapHelper (f : α → β) (arr : Array α) (soFar : Array β) (i : Fin arr.size) : Array β :=
+    let nextAccum := soFar.push (f arr[i])
+    if h : i.val + 1 < arr.size then
+      have : Array.size arr - (i.val + 1) < Array.size arr - i.val := by
+        apply Nat.sub_succ_lt_self
+        exact i.isLt
+      arrayMapHelper f arr nextAccum ⟨i + 1, h⟩
+    else
+      nextAccum
+  termination_by arrayMapHelper _ arr _ i => arr.size - i.val
+
+
+  def Array.map (f : α → β) (arr : Array α) : Array β :=
+    if h : arr.size > 0 then
+      arrayMapHelper f arr Array.empty ⟨0, h⟩
+    else
+      Array.empty
+end Finny
